more duplicate instance bounds

Batteries/Data/Iterators/Scan.lean
@@ -70,7 +70,7 @@ inductive IsPlausibleStep (it : IterM (α := ScanM α m f) n γ) :
       it.internalState.inner.IsPlausibleStep .done →
       IsPlausibleStep it .done
 
-instance instIterator [MonadLiftT m n] : Iterator (ScanM α m f) n γ where
+instance instIterator : Iterator (ScanM α m f) n γ where
   IsPlausibleStep := ScanM.IsPlausibleStep
   step it := do
       if h : it.internalState.yieldAcc = true then
@@ -94,18 +94,15 @@ instance instIterator [MonadLiftT m n] : Iterator (ScanM α m f) n γ where
           pure <| .deflate <| .done (by exact .done (by simpa using h) hp)
 
 namespace Finite
-private def Rel [Monad m] [Monad n] [Finite α m] :
-    IterM (α := ScanM α m f) n γ → IterM (α := ScanM α m f) n γ → Prop :=
+private def Rel [Finite α m] : IterM (α := ScanM α m f) n γ → IterM (α := ScanM α m f) n γ → Prop :=
   InvImage
     (Prod.Lex
       (· < ·)
       IterM.IsPlausibleSuccessorOf)
     (fun it => (it.internalState.yieldAcc.toNat, it.internalState.inner))
 
-private theorem Rel.of_yieldAcc [Finite α m]
-    {it it' : IterM (α := ScanM α m f) n γ}
-    (h' : it'.internalState.yieldAcc = false)
-    (h : it.internalState.yieldAcc = true) :
+private theorem Rel.of_yieldAcc [Finite α m] {it it' : IterM (α := ScanM α m f) n γ}
+    (h' : it'.internalState.yieldAcc = false) (h : it.internalState.yieldAcc = true) :
     Rel it' it := by
   apply Prod.Lex.left
   simp_all
@@ -117,7 +114,7 @@ private theorem Rel.of_inner [Finite α m]
     Rel it' it := by
   simp_all [Rel, InvImage, Prod.Lex.right]
 
-private def instFinitenessRelation [MonadLiftT m n] [Finite α m] :
+private def instFinitenessRelation [Finite α m] :
     FinitenessRelation (ScanM α m f) n where
   Rel := Rel
   wf := by
@@ -136,18 +133,17 @@ private def instFinitenessRelation [MonadLiftT m n] [Finite α m] :
     . exact IterM.isPlausibleSuccessorOf_of_skip ‹_›
 end Finite
 
-instance instFinite [Monad m] [Finite α m (β := β)] [Monad n] :
+instance instFinite [Finite α m (β := β)] :
     Finite (ScanM α m f) n :=
   .of_finitenessRelation Finite.instFinitenessRelation
 
-private def instProductivenessRelation [Monad m] [Monad n] [Productive α m] :
+private def instProductivenessRelation [Productive α m] :
     ProductivenessRelation (ScanM α m f) n where
   Rel := InvImage IterM.IsPlausibleSkipSuccessorOf (ScanM.inner ∘ IterM.internalState)
   wf := InvImage.wf _ Productive.wf
   subrelation h := by cases h; assumption
 
-instance instProductive [Monad m] [Monad n] [Productive α m] :
-    Productive (ScanM α m f) n :=
+instance instProductive [Productive α m] : Productive (ScanM α m f) n :=
   Productive.of_productivenessRelation instProductivenessRelation
 
 end ScanM
